Change the evaluation of modules with signatures
Restrict the module's environment to the values and constructors present
in the signature. This requires tracking the signature environment in
the evaluator's environment. We don't need to track the types, just
which variables and constructors are in the signature.

translator/ml_progScript.sml
@@ -28,18 +28,20 @@ val write_cons_def = zDefine `
     (env with c := nsAppend (nsSing n d) env.c)`
 
 val empty_env_def = zDefine `
-  (empty_env:v sem_env) = <| v := nsEmpty ; c:= nsEmpty|>`;
+  (empty_env:v sem_env) = <| v := nsEmpty ; c:= nsEmpty; s := nsEmpty |>`;
 
 val write_mod_def = zDefine `
   write_mod mn (env:v sem_env) env2 =
     env2 with <|
       c := nsAppend (nsLift mn env.c) env2.c
-      ; v := nsAppend (nsLift mn env.v) env2.v |>`
+      ; v := nsAppend (nsLift mn env.v) env2.v
+      ; s := nsAppend (nsLift mn env.s) env2.s |>`
 
 val merge_env_def = zDefine `
   merge_env (env2:v sem_env) env1 =
     <| v := nsAppend env2.v env1.v
-     ; c := nsAppend env2.c env1.c|>`
+     ; c := nsAppend env2.c env1.c
+     ; s := nsAppend env2.s env1.s|>`
 
 (* the components of nsLookup are 'nicer' partial functions *)
 
@@ -191,12 +193,16 @@ val write_conses_v = prove(
   ``!xs env. (write_conses xs env).v = env.v``,
   Induct \\ fs [write_conses_def,FORALL_PROD,write_cons_def]);
 
+val write_conses_s = prove(
+  ``!xs env. (write_conses xs env).s = env.s``,
+  Induct \\ fs [write_conses_def,FORALL_PROD,write_cons_def]);
+
 val write_tdefs_lemma = prove(
   ``!tds env n.
       write_tdefs n tds env =
-      merge_env <|v := nsEmpty; c := build_tdefs n tds|> env``,
+      merge_env <|v := nsEmpty; c := build_tdefs n tds; s := nsEmpty|> env``,
   Induct \\ fs [write_tdefs_def,merge_env_def,build_tdefs_def,FORALL_PROD]
-  \\ rw [write_conses_v]
+  \\ rw [write_conses_v, write_conses_s]
   \\ rewrite_tac [GSYM namespacePropsTheory.nsAppend_assoc]
   \\ AP_TERM_TAC
   \\ Q.SPEC_TAC (`REVERSE (build_constrs n p_2)`,`xs`)
@@ -204,7 +210,7 @@ val write_tdefs_lemma = prove(
 
 Theorem write_tdefs_thm
   `write_tdefs n tds empty_env =
-    <|v := nsEmpty; c := build_tdefs n tds|>`
+    <|v := nsEmpty; c := build_tdefs n tds; s := nsEmpty|>`
   (fs [write_tdefs_lemma,empty_env_def,merge_env_def]);
 
 val merge_env_write_conses = prove(
@@ -377,14 +383,16 @@ Theorem Decls_Dletrec
   \\ pop_assum (assume_tac o GSYM) \\ fs []);
 
 Theorem Decls_Dmod
-  `Decls env1 s1 [Dmod mn sn ds] env2 s2 <=>
+  `Decls env1 s1 [Dmod mn NONE ds] env2 s2 <=>
    ?s env.
       Decls env1 s1 ds env s /\ s2 = s /\
       env2 = write_mod mn env empty_env`
   (fs [Decls_def,Decls_def,evaluate_decs_def,PULL_EXISTS,
-      combine_dec_result_def,write_mod_def,empty_env_def]
+      combine_dec_result_def,write_mod_def,empty_env_def,
+      evaluateTheory.get_sig_names_def]
   \\ rw [] \\ eq_tac \\ rw [] \\ fs [pair_case_eq,result_case_eq]
-  \\ rveq \\ fs [] \\ asm_exists_tac \\ fs []);
+  \\ rveq \\ fs [] \\ asm_exists_tac \\ fs [] >>
+  metis_tac [nsRestrict_ident]);
 
 Theorem Decls_Dlocal
   `Decls env st lds env2 st2
