semantics/namespaceScript.sml
@@ -145,13 +145,13 @@ val _ = Define `
 
 (*val nsDom : forall 'v 'm 'n. Eq 'm, Eq 'n, Eq 'v, SetType 'v => namespace 'm 'n 'v -> set (id 'm 'n)*)
 val _ = Define `
- ((nsDom:('m,'n,'v)namespace ->(('m,'n)id)set) env=
+ ((nsDom:('m,'n,'v)namespace ->(('m,'n)id)set) env= 
   ({ n | v,n | (v IN UNIV) /\ (n IN UNIV) /\ (nsLookup env n = SOME v) }))`;
 
 
 (*val nsDomMod : forall 'v 'm 'n. SetType 'm, Eq 'm, Eq 'n, Eq 'v => namespace 'm 'n 'v -> set (list 'm)*)
 val _ = Define `
- ((nsDomMod:('m,'n,'v)namespace ->('m list)set) env=
+ ((nsDomMod:('m,'n,'v)namespace ->('m list)set) env= 
   ({ n | v,n | (v IN UNIV) /\ (n IN UNIV) /\ (nsLookupMod env n = SOME v) }))`;
 
 
@@ -162,4 +162,14 @@ val _ = Define `
        (MAP (\ (mn,e) .  (mn, nsMap f e)) m)))`;
 
 val _ = Lib.with_flag (computeLib.auto_import_definitions, false) Defn.save_defn nsMap_defn;
+
+(*val nsRestrict: forall 'm 'n 'v 'w. Eq 'n, Eq 'v, Eq 'w => namespace 'm 'n 'v -> namespace 'm 'n 'w -> namespace 'm 'n 'v*)
+ val _ = Define `
+ ((nsRestrict:('m,'n,'v)namespace ->('m,'n,'w)namespace ->('m,'n,'v)namespace) (Bind v m) (Bind v' m')=
+   (Bind
+    (FILTER (\ (n,x) .  ~ ((ALOOKUP v' n) = NONE)) v)
+    m))`;
+
+
 val _ = export_theory()
+
